fairneris/examples/no_drop_dup.v
@@ -1,0 +1,108 @@
+From iris.proofmode Require Import proofmode.
+From trillium.program_logic Require Import ectx_lifting.
+From fairneris Require Import model_draft.
+From fairneris.aneris_lang Require Import aneris_lang.
+From fairneris.aneris_lang.state_interp Require Import state_interp state_interp_events.
+From fairneris.aneris_lang.program_logic Require Import aneris_weakestpre.
+
+Definition Aprog shA : expr :=
+  SendTo #(LitSocket shA) #"Hello" #saB.
+
+Definition Bprog shB : expr :=
+  ReceiveFrom #(LitSocket shB).
+
+Section with_Σ.
+  Context `{anerisG (fair_model_to_model simple_fair_model) Σ}.
+
+  Lemma wp_A shA :
+    {{{ shA ↪[ip_of_address saA] sA ∗ saA ⤳ (∅,∅) ∗ saB ⤇ (λ _, True) }}}
+      Aprog shA @[ip_of_address saA]
+    {{{ v, RET #v; True }}}.
+  Proof.
+    iIntros (Φ) "(Hsh & Hrt & Hmsg) HΦ".
+    rewrite aneris_wp_eq /aneris_wp_def.
+    iIntros (tid) "Hnode".
+    iApply wp_lift_atomic_head_step_no_fork; [done|].
+    iIntros (ex atr K tp1 tp2 σ Hexvalid Hex Hlocale) "(Hevs & Hσ & %Hvalid & Hauth) /=".
+    iMod (steps_auth_update_S with "Hauth") as "Hauth".
+    rewrite (last_eq_trace_ends_in _ _ Hex).
+    iDestruct (aneris_state_interp_socket_valid with "Hσ Hsh")
+      as (Sn r) "[%HSn (%Hr & %Hreset)]".
+    iSplitR.
+    { iPureIntro; do 3 eexists. eapply SocketStepS; eauto.
+        by econstructor; naive_solver. }
+    iModIntro.
+    iIntros (v2' ? ? Hstep).
+    pose proof (λ b c d f g h i j k,
+                aneris_events_state_interp_send_untracked {[saA]} b c d f g h _ i _ _ _ _ (inl (ip_of_address saA,tid)) j k Hstep)
+      as Huntracked.
+    inv_head_step; iNext.
+    rewrite (insert_id (state_sockets σ)); last done.
+    rewrite (insert_id (state_sockets σ)) in Huntracked; last done.
+    iAssert (socket_address_group_own {[saA]})%I as "#HsaA".
+    { iDestruct "Hrt" as "[(%send & %recv & _ & _ & _ & $ & _) _]". }
+        iAssert (socket_address_group_own {[saB]})%I as "#HsaB".
+    { by iDestruct "Hmsg" as (γ) "[H _]". }
+    iMod (aneris_state_interp_send shA saA {[saA]} saB {[saB]} _ _ sA _ _ _ _ _
+                                   "Hello"
+           with "[] [] [$Hsh] [Hrt] [$Hmsg] [] [$Hσ]")
+        as "(%Hmhe & Hσ & Hsh & Hrt)";
+      [try set_solver..|].
+    { apply message_group_equiv_refl; set_solver. }
+    { iFrame "#". iPureIntro; set_solver. }
+    { iFrame "#". iPureIntro; set_solver. }
+    { iDestruct "Hrt" as "[$ Hrt]". }
+    { simpl. rewrite /from_singleton. eauto. }
+    (* Derive this using ghost state tracking current live roles *)
+    assert (A ∈ simple_live_roles (trace_last atr)) as Hrole by admit.
+    assert ((trace_last atr) = model_draft.Start) as Heq.
+    { destruct (trace_last atr); simpl in Hrole; set_solver. }
+    iExists (Sent 1), (Some A).
+    iDestruct (Huntracked with "Hrt Hevs") as "[$ Hrt]";
+          [done..|set_solver|].
+    iModIntro.
+    rewrite -Hmhe.
+    iFrame.
+    iSplitR; [done|].
+    simpl.
+    iSpecialize ("HΦ" with "[//]").
+    iSplitR "HΦ"; [|by iExists _; iFrame].
+    iPureIntro.
+    rewrite /simple_valid_state_evolution in Hvalid.
+    rewrite /simple_valid_state_evolution.
+    rewrite Heq in Hvalid. simpl in Hvalid.
+    simpl.
+    destruct Hvalid as [Hms Hskt].
+    rewrite /trace_ends_in in Hex.
+    rewrite Hex in Hms. simpl in Hms. rewrite Hms.
+    split.
+    { rewrite (comm _ ∅). f_equiv. f_equiv. eauto. }
+    rewrite Hex in Hskt.
+    simpl in Hskt.
+    done.
+  Admitted.
+
+  Lemma wp_B shB :
+    {{{ shB ↪[ip_of_address saB] sB ∗ saB ⤳ (∅,∅) ∗ saB ⤇ (λ _, True) }}}
+      Bprog shB @[ip_of_address saA]
+    {{{ v, RET v; True }}}.
+  Proof.
+    iIntros (Φ) "(Hsh & Hrt & #HΨ) HΦ".
+    rewrite aneris_wp_eq /aneris_wp_def.
+    iIntros (tid) "Hnode".
+    iLöb as "IH".
+    iApply wp_lift_head_step; auto.
+    iIntros (ex atr K tp1 tp2 σ Hexvalid Hex) "(Hevs & Hσ & Hm & Hauth) /=".
+    iMod (steps_auth_update_S with "Hauth") as "Hauth".
+    rewrite (last_eq_trace_ends_in _ _ Hex).
+    iDestruct (aneris_state_interp_socket_valid with "Hσ Hsh")
+      as (Sn r) "[%HSn (%Hr & %Hreset)]".
+    iMod (fupd_mask_intro_subseteq _ ∅ True%I with "[]") as "Hmk";
+      first set_solver; auto.
+    iModIntro. iSplitR.
+    { iPureIntro. admit. }
+    iIntros (v2' ? ? Hstep).
+    admit.
+  Admitted.
+
+End with_Σ.
